synchronized bfn and bfr with the new bft_std & bft_forest & bft_fifo

fifo.v
@@ -10,26 +10,24 @@
 (**************************************************************)
 
 Require Import bt List.
-Require fifo_axm.
-Require fifo_triv.
-Require fifo_2lists.
-Require fifo_3llists.
+
+Require fifo_axm fifo_triv fifo_2lists fifo_3llists.
 
 Set Implicit Arguments.
 
 Module Type FIFO.
 
-Parameters (fifo      : Type -> Type)
-           (fifo_list : forall X, fifo X -> list X)
-           (fifo_nil  : forall X, { q : fifo X | fifo_list q = nil })
-           (fifo_enq  : forall X q x, { q' : fifo X | fifo_list q' = fifo_list q ++ x :: nil })
-           (fifo_deq  : forall X q, @fifo_list X q <> nil -> { c : X * fifo X | let (x,q') := c in fifo_list q = x::fifo_list q' })
-           (fifo_void : forall X q, { b : bool | b = true <-> @fifo_list X q = nil }).
+  Parameters (fifo    : Type -> Type)
+             (tolist  : forall X, fifo X -> list X)
+             (empty   : forall X, { q : fifo X | tolist q = nil })
+             (enq     : forall X q x, { q' : fifo X | tolist q' = tolist q ++ x :: nil })
+             (deq     : forall X q, @tolist X q <> nil -> { c : X * fifo X | let (x,q') := c in tolist q = x::tolist q' })
+             (void    : forall X q, { b : bool | b = true <-> @tolist X q = nil }).
 
-Arguments fifo_nil {X}.
-Arguments fifo_deq {X}.
+(*  Arguments empty {X}.
+  Arguments deq {X}. *)
 
-Notation fifo_lsum := ((fun X (q : fifo (bt X)) => lsum (fifo_list q)) _).
+  Notation fifo_lsum := ((fun X (q : fifo (bt X)) => lsum (tolist q)) _).
 
 End FIFO.
 
@@ -37,11 +35,11 @@ End FIFO.
 Module FIFO_triv <: FIFO.
 
   Definition fifo := fifo_triv.fifo.
-  Definition fifo_list := fifo_triv.fifo_list.
-  Definition fifo_nil (X: Type) := fifo_triv.fifo_nil (X:=X).
-  Definition fifo_enq := fifo_triv.fifo_enq.
-  Definition fifo_deq (X: Type) := fifo_triv.fifo_deq (X:=X).
-  Definition fifo_void := fifo_triv.fifo_void.
+  Definition tolist := fifo_triv.fifo_list.
+  Definition empty := @fifo_triv.fifo_nil.
+  Definition enq := fifo_triv.fifo_enq.
+  Definition deq := @fifo_triv.fifo_deq.
+  Definition void := fifo_triv.fifo_void.
 
 End FIFO_triv.
 
@@ -49,11 +47,11 @@ End FIFO_triv.
 Module FIFO_2lists <: FIFO.
 
   Definition fifo := fifo_2lists.fifo.
-  Definition fifo_list := fifo_2lists.fifo_list.
-  Definition fifo_nil (X: Type) := fifo_2lists.fifo_nil (X:=X).
-  Definition fifo_enq := fifo_2lists.fifo_enq.
-  Definition fifo_deq (X: Type) := fifo_2lists.fifo_deq (X:=X).
-  Definition fifo_void := fifo_2lists.fifo_void.
+  Definition tolist := fifo_2lists.fifo_list.
+  Definition empty := @fifo_2lists.fifo_nil.
+  Definition enq := fifo_2lists.fifo_enq.
+  Definition deq := @fifo_2lists.fifo_deq.
+  Definition void := fifo_2lists.fifo_void.
 
 End FIFO_2lists.
 
@@ -61,11 +59,11 @@ End FIFO_2lists.
 Module FIFO_3llists <: FIFO.
 
   Definition fifo := fifo_3llists.fifo.
-  Definition fifo_list := fifo_3llists.fifo_list.
-  Definition fifo_nil (X: Type) := fifo_3llists.fifo_nil (X:=X).
-  Definition fifo_enq := fifo_3llists.fifo_enq.
-  Definition fifo_deq (X: Type) := fifo_3llists.fifo_deq (X:=X).
-  Definition fifo_void := fifo_3llists.fifo_void.
+  Definition tolist := fifo_3llists.fifo_list.
+  Definition empty := @fifo_3llists.fifo_nil.
+  Definition enq := fifo_3llists.fifo_enq.
+  Definition deq := @fifo_3llists.fifo_deq.
+  Definition void := fifo_3llists.fifo_void.
 
 End FIFO_3llists.
 
@@ -73,10 +71,10 @@ End FIFO_3llists.
 Module FIFO_axm <: FIFO.
 
   Definition fifo := fifo_axm.fifo.
-  Definition fifo_list := fifo_axm.fifo_list.
-  Definition fifo_nil (X: Type) := fifo_axm.fifo_nil (X:=X).
-  Definition fifo_enq := fifo_axm.fifo_enq.
-  Definition fifo_deq (X: Type) := fifo_axm.fifo_deq (X:=X).
-  Definition fifo_void := fifo_axm.fifo_void.
+  Definition tolist := fifo_axm.fifo_list.
+  Definition empty := @fifo_axm.fifo_nil.
+  Definition enq := fifo_axm.fifo_enq.
+  Definition deq := @fifo_axm.fifo_deq.
+  Definition void := fifo_axm.fifo_void.
 
 End FIFO_axm.
