bfn_fifo.v
@@ -18,18 +18,30 @@
 
 *)
 
+(** We exploit the following equations from bft_forest to 
+    get an efficient implementation with queues ... this
+    corresponds to bftrav' in Okazaki's paper
+
+    See bft_forest.v for the proofs 
+
+    Corollary bft_f_fix_oka_0 : bft_f nil = nil.
+    Corollary bft_f_fix_oka_1 x l : bft_f (leaf x::l) = x::bft_f l.
+    Corollary bft_f_fix_oka_2 a x b l : bft_f (node a x b::l) = x::bft_f (l++a::b::nil).
+
+*)
+
 Require Import List Arith Omega Extraction.
 
-Require Import list_utils wf_utils.
-Require Import bt bft fifo.
+Require Import list_utils wf_utils bt fifo bft_forest bft_std.
 
 Set Implicit Arguments.
 
 Module BFN_FIFO (M: FIFO).
 
-  Export M.
+Export M.
 
-  Section bfn_fifo.
+Section bfn_fifo.
+
   Variable (X : Type).
 
   (* the forest (list of bt nat) is a breadth first numbering from n if
@@ -118,39 +130,39 @@ Module BFN_FIFO (M: FIFO).
 
   Implicit Type p : fifo (bt X).
 
-  Definition bfn_fifo_f n p : { q | fifo_list p ~lt rev (fifo_list q) /\ is_bfn_from n (rev (fifo_list q)) }.
+  Definition bfn_fifo_f n p : { q | tolist p ~lt rev (tolist q) /\ is_bfn_from n (rev (tolist q)) }.
   Proof.
     induction on n p as bfn_fifo_f with measure (fifo_lsum p).
 
-    refine (let (b,Hb) := fifo_void p in _).
+    refine (let (b,Hb) := void p in _).
     revert Hb; refine (match b with 
       | true  => fun Hp 
-      => let (q,Hq) := fifo_nil 
+      => let (q,Hq) := @empty _ 
          in exist _ q _
       | false => fun Hp 
-      => let (d1,Hd1) := @fifo_deq _ p _ 
+      => let (d1,Hd1) := @deq _ p _ 
          in _
     end). 
     all: cycle 2. (* We queue 2 POs *)
     revert Hd1; refine (match d1 with
       | (leaf x    , p1) => fun Hp1 
-      => let (q,Hq)   := bfn_fifo_f (S n) p1 _           in
-         let (q1,Hq1) := fifo_enq q (leaf n) 
+      => let (q,Hq)   := bfn_fifo_f (S n) p1 _     in
+         let (q1,Hq1) := enq q (leaf n) 
          in  exist _ q1 _
       | (node a x b, p1) => fun Hp1 
-      => let (p2,Hp2) := fifo_enq p1 a                  in
-         let (p3,Hp3) := fifo_enq p2 b                  in
-         let (q,Hq)   := bfn_fifo_f (S n) p3 _           in 
-         let (d2,Hd2) := @fifo_deq _ q _ 
+      => let (p2,Hp2) := enq p1 a                  in
+         let (p3,Hp3) := enq p2 b                  in
+         let (q,Hq)   := bfn_fifo_f (S n) p3 _     in 
+         let (d2,Hd2) := @deq _ q _ 
          in  _
     end); simpl in Hp1.
     all: cycle 4. (* We queue 4 POs *)
     revert Hd2; refine (match d2 with (u,q1) => _ end); intros Hq1.
-    refine (let (d3,Hd3) := @fifo_deq _ q1 _ in _).
+    refine (let (d3,Hd3) := @deq _ q1 _ in _).
     all: cycle 1. (* We queue 1 PO *) 
     revert Hd3; refine (match d3 with 
       | (v,q2) => fun Hq2 
-      => let (q3,Hq3) := fifo_enq q2 (node v n u)
+      => let (q3,Hq3) := enq q2 (node v n u)
          in  exist _ q3 _
     end); simpl in Hq2, Hq3.
     all: cycle 1. (* We queue 1 PO *) 
@@ -158,14 +170,14 @@ Module BFN_FIFO (M: FIFO).
     (* And now, we show POs *)
    
     * apply proj1 in Hp; rewrite Hp, Hq; split; simpl; auto.
-      red; rewrite bft_f_fix_0; simpl; auto.
+      red; rewrite bft_f_fix_oka_0; simpl; auto.
     * intros H; apply Hp in H; discriminate.
     * rewrite Hp1; simpl; omega.
     * destruct Hq as (H5 & H6).
       rewrite Hp1, Hq1; split; auto.
       + rewrite rev_app_distr; simpl; auto.
       + rewrite rev_app_distr; simpl; red.
-        rewrite bft_f_fix_3; simpl; rewrite <- app_nil_end; auto.
+        rewrite bft_f_fix_oka_1; simpl; auto.
     * rewrite Hp3, Hp2, app_ass; simpl.
       rewrite lsum_app, Hp1; simpl; omega.
     * apply proj1, Forall2_rev in Hq; intros H; revert Hq.
@@ -184,19 +196,19 @@ Module BFN_FIFO (M: FIFO).
       rewrite Hq1, Hq2 in H6; simpl in H6; rewrite app_ass in H6; simpl in H6.
       unfold is_bfn_from in H6 |- *.
       rewrite Hp1, Hq3, rev_app_distr; simpl.
-      rewrite bft_f_fix_3; simpl; split; auto.
+      rewrite bft_f_fix_oka_2; simpl; auto.
   Defined.
 
   Section bfn.
 
     Implicit Type (t : bt X).
 
-    Let bfn_fifo_full t : { t' | t ~t t' /\ is_seq_from 0 (bft_std t') }.
+    Let bfn_fifo_full t : { t' | t ~t t' /\ is_seq_from 0 (bft_forest t') }.
     Proof.
-      refine (let (p,Hp) := @fifo_nil _   in
-              let (q,Hq) := fifo_enq p t  in 
+      refine (let (p,Hp) := @empty _       in
+              let (q,Hq) := enq p t        in 
               let (r,Hr) := bfn_fifo_f 0 q in
-              let (d1,Hd1) := @fifo_deq _ r _ 
+              let (d1,Hd1) := @deq _ r _ 
               in _).
       all: cycle 1. (* We queue 1 PO *) 
       revert Hd1; refine (match d1 with (x,q1) => fun Hq1 => exist _ x _ end); simpl in Hq1.
@@ -206,7 +218,6 @@ Module BFN_FIFO (M: FIFO).
         apply proj1 in Hr; inversion Hr.
       * rewrite Hq, Hp in Hr. 
         destruct Hr as (H1 & H2).
-        rewrite <- bft_eq_bft_std.
         rewrite Hq1 in H1; simpl in H1.
         apply Forall2_snoc_inv with (l := nil) in H1.
         destruct H1 as (G1 & H1).
@@ -223,7 +234,11 @@ Module BFN_FIFO (M: FIFO).
     Proof. apply (proj2_sig (bfn_fifo_full t)). Qed.
 
     Fact bfn_fifo_spec_2 t : exists n, bft_std (bfn_fifo t) = seq_an 0 n.
-    Proof. apply is_seq_from_spec, (proj2_sig (bfn_fifo_full t)). Qed.
+    Proof. 
+      apply is_seq_from_spec.
+      rewrite <- bft_forest_eq_bft_std. 
+      apply (proj2_sig (bfn_fifo_full t)). 
+    Qed.
 
     Corollary bfn_fifo_spec_3 t : bft_std (bfn_fifo t) = seq_an 0 (m_bt t).
     Proof.
@@ -243,5 +258,6 @@ End bfn_fifo.
 Check bfn_fifo.
 Check bfn_fifo_spec_1.
 Check bfn_fifo_spec_2.
+Check bfn_fifo_spec_3.
 
 End BFN_FIFO.
