bft_fifo.v
@@ -9,32 +9,43 @@
 (*         CeCILL v2 FREE SOFTWARE LICENSE AGREEMENT          *)
 (**************************************************************)
 
-Require Import List Arith Omega Extraction.
+(** We exploit the following equations from bft_forest to 
+    get an efficient implementation with queues ... this
+    corresponds to bftrav' in Okazaki's paper
 
-Require Import list_utils wf_utils. 
-Require Import bt bft fifo.
+    See bft_forest.v for the proofs 
+
+    Corollary bft_f_fix_oka_0 : bft_f nil = nil.
+    Corollary bft_f_fix_oka_1 x l : bft_f (leaf x::l) = x::bft_f l.
+    Corollary bft_f_fix_oka_2 a x b l : bft_f (node a x b::l) = x::bft_f (l++a::b::nil).
+
+*)
+
+Require Import List Arith Omega.
+Require Import list_utils wf_utils bt fifo bft_std bft_forest.
 
 Set Implicit Arguments.
 
 Module BFT_FIFO (M: FIFO).
 
-  Export M.
+Export M.
 
-  Section bft_fifo.
+Section bft_fifo.
+
   Variable (X : Type).
 
   Implicit Type p : fifo (bt X). 
 
-  Definition bft_fifo_f p : { l | l = bft_f (fifo_list p) }.
+  Definition bft_fifo_f p : { l | l = bft_f (tolist p) }.
   Proof.
     induction on p as bft_fifo_f with measure (fifo_lsum p).
 
-    refine (let (b,Hb) := fifo_void p in _).
+    refine (let (b,Hb) := void p in _).
     revert Hb; refine (match b with 
       | true  => fun Hp 
       => exist _ nil _
       | false => fun Hp 
-      => let (c,Hc) := @fifo_deq _ p _ 
+      => let (c,Hc) := @deq _ p _ 
          in _
     end). 
     all: cycle 2. (* We queue 2 POs *)
@@ -44,8 +55,8 @@ Module BFT_FIFO (M: FIFO).
       => let (r,Hr) := bft_fifo_f q _ 
          in  exist _ (x::r) _
       | node a x b => fun Hq 
-      => let (r,Hr) := fifo_enq q a    in
-         let (s,Hs) := fifo_enq r b    in
+      => let (r,Hr) := enq q a    in
+         let (s,Hs) := enq r b    in
          let (t,Ht) := bft_fifo_f s _
          in  exist _ (x::t) _
     end); simpl in Hq.
@@ -54,25 +65,20 @@ Module BFT_FIFO (M: FIFO).
     (* And now, we show POs *)
    
     * rewrite (proj1 Hp); auto.
-      rewrite bft_f_fix_0; reflexivity.
+      rewrite bft_f_fix_oka_0; reflexivity.
     * intros H; apply Hp in H; discriminate.
     * rewrite Hq; simpl; auto.
-    * rewrite Hr, Hq.
-      rewrite bft_f_fix_3; simpl.
-      do 2 f_equal; apply app_nil_end.
+    * rewrite Hr, Hq, bft_f_fix_oka_1; auto.
     * rewrite Hs, Hr, Hq; simpl.
       do 2 rewrite lsum_app; simpl; omega.
-    * rewrite Ht, Hs, Hr, Hq.
-      rewrite app_ass; simpl.
-      rewrite bft_f_fix_3, bft_f_fix_1; simpl.
-      rewrite bft_f_fix_1; auto.
+    * rewrite Ht, Hs, Hr, Hq, bft_f_fix_oka_2, app_ass; auto.
   Defined.
 
-  Let bft_fifo_full t : { l : list X | l = bft t }.
+  Let bft_fifo_full t : { l : list X | l = bft_forest t }.
   Proof.
     refine (
-      let (q0,H0) := @fifo_nil _   in
-      let (q1,H1) := fifo_enq q0 t in
+      let (q0,H0) := empty _       in
+      let (q1,H1) := enq q0 t      in
       let (l,Hl)  := bft_fifo_f q1   
       in  exist _ l _).
     rewrite Hl, H1, H0; reflexivity.
@@ -80,12 +86,14 @@ Module BFT_FIFO (M: FIFO).
 
   Definition bft_fifo t := proj1_sig (bft_fifo_full t).
 
-  Fact bft_fifo_spec t : bft_fifo t = bft t.
-  Proof. apply (proj2_sig (bft_fifo_full t)). Qed.
+  Theorem bft_fifo_spec t : bft_fifo t = bft_std t.
+  Proof. 
+    rewrite <- bft_forest_eq_bft_std.
+    apply (proj2_sig (bft_fifo_full t)). 
+  Qed.
 
 End bft_fifo.
 
-Check bft_fifo.
 Check bft_fifo_spec.
 
 End BFT_FIFO.
