extraction.v
@@ -10,7 +10,7 @@
 (**************************************************************)
 
 Require Import List Extraction.
-Require Export bt fifo bft bft_fifo bfn_fifo bfr_fifo.
+Require Export bt fifo bft_std bft_forest bft_fifo bfn_fifo bfr_fifo.
 
 Extract Inductive bool => "bool" [ "true" "false" ].
 Extract Inductive prod => "(*)"  [ "(,)" ].
@@ -18,24 +18,29 @@ Extract Inductive list => "list" [ "[]" "(::)" ].
 Extract Inductive nat => int [ "0" "succ" ] "(fun fO fS n -> if n=0 then fO () else fS (n-1))".
 
 Module BFT_triv := BFT_FIFO FIFO_triv.
-Module BFN_triv := BFN_FIFO FIFO_triv.
-Module BFR_triv := BFR_FIFO FIFO_triv.
-
 Module BFT_2lists := BFT_FIFO FIFO_2lists.
-Module BFN_2lists := BFN_FIFO FIFO_2lists.
-Module BFR_2lists := BFR_FIFO FIFO_2lists.
-
 Module BFT_3llists := BFT_FIFO FIFO_3llists.
-Module BFN_3llists := BFN_FIFO FIFO_3llists.
-Module BFR_3llists := BFR_FIFO FIFO_3llists.
-
-(** the following does not yield executable extracted programs *)
 Module BFT_axm := BFT_FIFO FIFO_axm.
+
+Module BFN_triv := BFN_FIFO FIFO_triv.
+Module BFN_2lists := BFN_FIFO FIFO_2lists.
+Module BFN_3llists := BFN_FIFO FIFO_3llists.
 Module BFN_axm := BFN_FIFO FIFO_axm.
+
+Module BFR_triv := BFR_FIFO FIFO_triv.
+Module BFR_2lists := BFR_FIFO FIFO_2lists.
+Module BFR_3llists := BFR_FIFO FIFO_3llists.
 Module BFR_axm := BFR_FIFO FIFO_axm.
 
+Recursive Extraction BFT_triv.bft_fifo BFT_2lists.bft_fifo BFT_3llists.bft_fifo.
+Recursive Extraction BFN_triv.bfn_fifo BFN_2lists.bfn_fifo BFN_3llists.bfn_fifo.
+Recursive Extraction BFR_triv.bfr_fifo BFR_2lists.bfr_fifo BFR_3llists.bfr_fifo.
 
-Recursive Extraction BFT_triv.bft_fifo
+(** the following does not yield executable extracted programs *)
+
+
+
+(*Recursive Extraction BFT_triv.bft_fifo
                      BFN_triv.bfn_fifo
                      BFR_triv.bfr_fifo.
 
@@ -51,3 +56,4 @@ Recursive Extraction BFT_axm.bft_fifo
                      BFN_axm.bfn_fifo
                      BFR_axm.bfr_fifo.
 
+*)
